backend/PrintAnnot.ml
@@ -1,0 +1,76 @@
+(* *********************************************************************)
+(*                                                                     *)
+(*              The Compcert verified compiler                         *)
+(*                                                                     *)
+(*          Xavier Leroy, INRIA Paris-Rocquencourt                     *)
+(*                                                                     *)
+(*  Copyright Institut National de Recherche en Informatique et en     *)
+(*  Automatique.  All rights reserved.  This file is distributed       *)
+(*  under the terms of the INRIA Non-Commercial License Agreement.     *)
+(*                                                                     *)
+(* *********************************************************************)
+
+(* Printing annotations in asm syntax *)
+
+open Printf
+open Datatypes
+open Integers
+open Floats
+open Camlcoq
+open AST
+open Memdata
+open Asm
+
+let re_annot_param = Str.regexp "%%\\|%[1-9][0-9]*"
+
+type arg_value =
+  | Reg of preg
+  | Stack of memory_chunk * Int.int
+  | Intconst of Int.int
+  | Floatconst of float
+
+let print_annot_text print_preg sp_reg_name oc txt args =
+  let print_fragment = function
+  | Str.Text s ->
+      output_string oc s
+  | Str.Delim "%%" ->
+      output_char oc '%'
+  | Str.Delim s ->
+      let n = int_of_string (String.sub s 1 (String.length s - 1)) in
+      try
+        match List.nth args (n-1) with
+        | Reg r ->
+            print_preg oc r
+        | Stack(chunk, ofs) ->
+            fprintf oc "mem(%s + %ld, %ld)"
+               sp_reg_name
+               (camlint_of_coqint ofs)
+               (camlint_of_coqint (size_chunk chunk))
+        | Intconst n ->
+            fprintf oc "%ld" (camlint_of_coqint n)
+        | Floatconst n ->
+            fprintf oc "%.18g" (camlfloat_of_coqfloat n)
+      with Failure _ ->
+        fprintf oc "<bad parameter %s>" s in
+  List.iter print_fragment (Str.full_split re_annot_param txt);
+  fprintf oc "\n"
+
+let rec annot_args tmpl args =
+  match tmpl, args with
+  | [], _ -> []
+  | AA_arg _ :: tmpl', APreg r :: args' ->
+      Reg r :: annot_args tmpl' args'
+  | AA_arg _ :: tmpl', APstack(chunk, ofs) :: args' ->
+      Stack(chunk, ofs) :: annot_args tmpl' args'
+  | AA_arg _ :: tmpl', [] -> []         (* should never happen *)
+  | AA_int n :: tmpl', _ ->
+      Intconst n :: annot_args tmpl' args
+  | AA_float n :: tmpl', _ ->
+      Floatconst n :: annot_args tmpl' args
+
+let print_annot_stmt print_preg sp_reg_name oc txt tmpl args =
+  print_annot_text print_preg sp_reg_name oc txt (annot_args tmpl args)
+
+let print_annot_val print_preg oc txt args =
+  print_annot_text print_preg "<internal error>" oc txt
+    (List.map (fun r -> Reg r) args)
